# 2.2 ‚Äì Evaluating Expressions {.unnumbered}

In the last lesson, you learned how to **read** and **write** algebraic expressions -- the "phrases" of math. As with any language, the meaning of phrases can change with the situation. This is true in algebra too! The meaning or **value** of an expression depends on what numbers we use for its variables. 

In this lesson, we will learn to **substitute** numbers for the variables in an expression so that we can **evaluate** its meaning in a particular situation.

---

:::{.objectives}
- I can substitute values into expressions and simplify them  
- I can use the correct order of operations with variables and parentheses  
- I can use substitution to show two expressions are equivalent
:::

---

:::{.vocab}
{{< glink evaluate >}}, {{< glink expression >}}, {{< glink operation >}}, {{< glink result >}}, {{< glink value >}}, {{< glink variable >}}

:::

---

## üî• Warm-Up

1. What do you get if you simplify this expression?  
   $$
   3 + 2 \cdot 4
   $$

2. In what ways are $2x + 5$ and $5 + 2x$ different? In what ways are they the same?

3. A student evaluates $(-3)^2$ and gets -9. Are they correct? Why or why not?

---

## üë• Learn Together

### 2.2.1 ‚Äì What Does It Mean to Evaluate?

To **evaluate** an {{< glink expression >}} means to find its {{< glink value >}} by **substituting** (replacing) the variable with a number.

**Example 1:**

Evaluate $4x + 1$ when $x = 3$.

First we replace the $x$ with what it is.

$$
4(\color{red}3\color{black}) + 1
$$

Now we simplify (or {{< glink calculate >}}) the {{< glink result >}}.

$$
4(3) + 1 = 12 + 1 = 13
$$

:::{.remember}
When you see "**=**", think "**is**". In the previous example, we could say "x **is** 3".
:::

**Example 2:**

Evaluate $3 - 2x$ when $x = -4$.

First substitute.

$$
3 - 2(\color{red}{-4}\color{black})
$$

Then simplify.

$$
3 - 2(-4) = 3 + 8 = 11
$$

:::{.gotcha}
It is easy to lose track of negative signs when substituting numbers in an expression. To avoid mistakes, put parentheses in place of the variable before substituting a number.
:::

:::{.you-try title="Evaluate $5x-2$ when $x=-3$"}

$$
5(\color{red}-3\color{black}) - 2 = -15 - 2 = -17
$$

:::

Now that you know how to evaluate an expression, let's try some more complicated ones that will require us to remember our {{< glink order of operations >}}.

---

### 2.2.2 ‚Äì Using PEMDAS with Substitution

Evaluating expressions is just one additional step on top of the order of operations. First we substitute, and then we apply {{< glink PEMDAS >}}. 

**Example 1:**

Evaluate $2(x + 3)^2$ when $x = 1$.

First we substitute.

$$
2((\color{red}{1}\color{black}) + 3)^2
$$

Then we simplify.

$$
2(1 + 3)^2 = 2(4)^2 = 2 \cdot 16 = 32
$$

**Example 2:**

Evaluating expressions works the same way if the variable shows up more than once. This expression has the variable $y$ in two places.

Evaluate $3(2 - y) + 5(y - 2)$ when $y=-4$.

Substitute:

$$
3(2 - (\color{red}{-4})\color{black}) + 5((\color{red}{-4}\color{black}) - 2)
$$

Now simplify:

$$
3(2 -(-4)) + 5((-4) - 2) = 3(6) + 5(-6) = 18 - 30 = -12
$$

:::{.you-try title="Evaluate $20(x - 2) + 2x^2$ when $x=5$."}

Substitute:
$$
20((\color{red}{5}\color{black}) - 2) + 2(\color{red}{5}\color{black})^2
$$

Simplify:

$$
20(5 - 2) + 2(5)^2 = 20(3) + 2(25) = 60 + 50 = 110
$$

:::

---

### 2.2.3 ‚Äì Evaluating Expressions With Multiple Variables

It may look more difficult, but there is no difference between evaluating expressions with one variable and evaluating them with 2 or more variables.

In the following example, we have the variables $a$ and $b$. 

**Example 1:**

Evaluate the expression $2a - 3b$ when $a=2$ and $b=1$.

We do exactly what we did in the previous examples. First we substitute for $\color{blue}{a}$ and $\color{red}{b}$:

$$
2(\color{blue}{2}\color{black}) - 3(\color{red}{1}\color{black})
$$

Then we simplify:

$$
2(2) - 3(1) = 4 - 3 = 1
$$


**Example 2:**

Evaluate $12x -3y^2$ when $x=7$ and $y=-3$.

First substitute for $\color{blue}{x}$ and $\color{red}{y}$. Be careful with the negatives!

$$
12(\color{blue}{7}\color{black}) - 3(\color{red}{-3}\color{black})^2
$$

Now we simplify:

$$
12(7) - 3(-3)^2 = 84 - 3(9) = 84 - 27 = 57
$$

:::{.you-try title="Evaluate $\frac{1}{2}x^2 - 3y$ when $x = 4$ and $y = 3$."}

First substitute for $\color{blue}{x}$ and $\color{red}{y}$.

$$
\frac{1}{2}(\color{blue}{4}\color{black})^2 - 3(\color{red}{3}\color{black})
$$

Now simplify:

$$
\frac{1}{2}(4)^2-3(3) = \frac{1}{2}(16)-9=8-9=-1
$$

:::

---

### 2.2.4 ‚Äì Testing For Equivalence

Sometimes two expressions look different but always give the same result. We call these {{< glink equivalent expressions >}}. 

To test for equivalence, we can substitute values into each expression and see if they give the same result.

**Example 1:**

Test if the expressions $5x - 25$ and $5(x - 5)$ are equivalent.

Let's try $x=9$:

$$
\begin{align*}
5(9) - 25 &= 45 - 25 &= 20 \\
5(9 - 5) &= 5(4) &= 20
\end{align*}
$$

They both gave the same result and so we have evidence that the two expressions are equivalent.

**Example 2:**

Test if expressions $3(x - 1)$ and $3x - 2$ are equivalent.

Let's try $x = 2$:

$$
\begin{align*}
3((2)-1) &= 3(1) &= 3 \\
3(2) - 2 &= 6 - 2 &= 4
\end{align*}
$$

These two expressions are **not** equivalent because they give different results when substituting the same number for $x$.

:::{.gotcha title="What does this prove?"}
When we substitute numbers to check if two expressions are equivalent, we are really testing a {{< glink hypothesis >}}:

- If the two expressions give **different results** for the same substitution, then they are **not equivalent**.

- If the two expressions give the **same result** for a substitution, that is **evidence** that they are equivalent, but it **does not** prove they are always the same.

**Example:**
Test if $6y$ and $2y$ are equivalent expressions.

Try $y = 0$.

$$
\begin{align*}
6(0) &= 0 \\
2(0) &= 0
\end{align*}
$$

We got the same result, so this is **evidence** that they could be equivalent. 

But what if we try $y=3$?

$$
\begin{align*}
6(3) &= 18 \\
2(3) &= 6
\end{align*}
$$

This proves that the expressions are **not equivalent**.

For now we can only test the hypothesis. In section 2.6 we will learn how to **prove** two expressions are equivalent.

:::

---

:::{.you-try-m title="Are they equivalent?"}

Test if $9y - 3$ is equivalent to $3(3y - 2) + 3$ using $y = 2$.

Did you get the same result? What does your answer tell you about the two expressions?

:::

:::{.answer title="Answer"}
If we substitute $y = 2$ we get:

$$
\begin{align*}
9(2) - 3 &= 18 - 3 &= 15 \\
3(3(2) - 2) + 3 &= 3(6 - 2) + 3 = 3(4) + 3 = 12 + 3 &= 15
\end{align*}
$$

We have evidence that the two expressions are equivalent but we don't know for certain. 

:::

---

## ‚úçÔ∏è Practice On Your Own

**Single variable**

1. Evaluate $3x + 4$ when $x=5$

2. Evaluate $7 - 2x$ when $x=-3$

3. Evaluate $2x^2$ when $x=2$

4. Evaluate $\frac{1}{2}x + 3$ when $x=6$

5. Evaluate $-x + 7$ when $x=-2$

---

**Single variable, repeated**

6. Evaluate $x + x + x$ when $x=4$

7. Evaluate $2x + 3x$ when $x=2$

8. Evaluate $x^2 + 3x^2$ when $x=1$

9. Evaluate $5x - 2x + 4$ when $x=3$

10. Evaluate $2(x+x) + 1$ when $x=-1$

---

**Parentheses / PEMDAS**

11. Evaluate $2(x+3)^2$ when $x=1$

12. Evaluate $3(x-2)^2 + 4$ when $x=3$

13. Evaluate $(2x+1)(x-1)$ when $x=2$

14. Evaluate $(x+2)^2 - 3x$ when $x=1$

15. Evaluate $\frac{3(x+4)}{2}$ when $x=2$

---

**Multiple variables**

16. Evaluate $2a - 3b$ when $a=3, b=5$

17. Evaluate $4x + 2y$ when $x=2, y=-1$

18. Evaluate $\frac{1}{2}x^2 - 3y$ when $x=4, y=3$

19. Evaluate $3x - 2y + z$ when $x=1, y=2, z=5$

20. Evaluate $(x+y)^2 - xy$ when $x=2, y=3$

---

**Testing Equivalence**

21. Are $2(x+3)$ and $2x+6$ equivalent? Test $x=4$

22. Are $4x + 2x$ and $6x$ equivalent? Test $x=-1$

23. Are $x^2 + 2x + 1$ and $(x+1)^2$ equivalent? Test $x=2$


---

**Challenge Problems**

24. Test if $3(a + b) - 2(a - b)$ and $a + 5b$ are equivalent. Try at least two different sets of values for $a$ and $b$.

25. Test if $2(a + b)^2 - 2a^2 - 4ab$ and $2b^2 are equivalent. Try at least two different sets of values for $a$ and $b$.

---

:::{.answers}
**Single variable**

1. 19

2. 13

3. 8

4. 6

5. 9

---

**Single variable, repeated**

6. 12

7. 10

8. 4

9. 13

10. -3

---

**Parentheses / PEMDAS**

11. 32

12. 7

13. 5

14. 6

15. 9

---

**Multiple variables**

16. -9

17. 6

18. -1

19. 4

20. 19

---

**Testing Equivalence**

21. evidence of equivalence

22. evidence of equivalence

23. evidence of equivalence

:::