# 2.4 – The Distributive Property {.unnumbered}

Imagine your football (soccer) team wants to order new jerseys. Each jersey costs $25, and to add your team’s logo it’s another $5 per jersey.

Since there are 11 players on the team, you need 11 jerseys. You could figure out the total cost in two different ways:

First, add the cost of one jersey and the logo: 25 + 5 = 30. Then multiply by 11 → 11 × 30 = $330.

Or multiply separately: (11 × 25) + (11 × 5) = 275 + 55 = $330.

Either way, you get the same answer. What we just did actually followed a rule in algebra called the {{< glink distributive property >}}. Today, we’re going to see how this property helps us simplify expressions.

---

:::{.objectives}

* I can use the **distributive property** to expand expressions like $a(b+c)$.
* I can distribute with **negatives** and then **combine like terms**.
* I can **factor out** a common factor (reverse distribution) to rewrite an expression.
:::

---

:::{.vocab}
{{< glink coefficient >}}, {{< glink distributive property >}}, {{< glink equivalent expressions >}}, {{< glink factor >}}, {{< glink greatest common factor >}}, {{< glink simplify >}}, {{< glink term >}}, {{< glink variable >}}
:::

---

## 🔥 Warm-Up

1. Mental math with parts:
   a) $6(10+4)$    b) $9(20-1)$    c) $5(3+0.2)$

2. True or false? Explain.
   a) $4(x+3)=4x+12$
   b) $4(x+3)=4x+3$

3. Which is easier to compute in your head? Why?
   a) $12 \times 25$ or $12(20+5)$
   b) $8 \times 19$ or $8(20-1)$

---

## 👥 Learn Together

### 2.4.1 – What Is the Distributive Property?

The **distributive property** says:

$$
a(b+c) = ab + ac \qquad\text{and}\qquad a(b-c)=ab-ac.
$$

Think of an **area model**. A rectangle with side lengths $(x+3)$ and $4$ can be split into two smaller rectangles: one $x$ by $4$ and one $3$ by $4$.

![](/images/Unit_2/Lesson_4/area_4_by_\(x+3\).png){width="420px"}

So the total area is $4x + 12$. That’s distribution in pictures.

**Examples**

1. $3(x+2)=3x+6$
2. $5(y-4)=5y-20$
3. $2(4a+3b)=8a+6b$

:::{.you-try-m title="Expand using the distributive property."}
a) $5(x+7)$
b) $2(3+y)$
c) $4(a+3b)$
d) $10(x-0.5)$
:::

:::{.answer title="Answer"}
a) $5x+35$    b) $6+2y$ or $2y+6$    c) $4a+12b$    d) $10x-5$
:::

---

### 2.4.2 – Distributing with Negatives

Careful with **signs**. The sign in front of the parentheses multiplies **every** term inside.

**Examples**

1. $-3(x-4) = -3x + 12$
2. $-(x+7)= -x - 7$ (think “$-1$ times each term”)
3. $6 - 2(x+3) = 6 - 2x - 6 = -2x$

:::{.gotcha title="Don’t skip a term"}
$4(x+2y+5)$ means $4x + 8y + 20$. Distribute to **every** term, not just the first two.
:::

:::{.you-try title="Expand and simplify $-2(3-y)+4(y+5)$"}

$$
-6 + 2y + 4y + 20 = 6y + 14
$$

:::

---

### 2.4.3 – Distribute, Then Combine Like Terms

We often distribute **and then** use what we learned in 2.3 (combine like terms).

**Example**

$$
4(x+2) + 3(x-5) = 4x + 8 + 3x - 15 = 7x - 7.
$$

Sometimes you can **simplify inside** first:

$$
2(x+3x-5)=2(4x-5)=8x-10,
$$

which is a little faster.

:::{.think title="Which path is better?"}
If you can combine inside the parentheses **first**, do it. If not, distribute and then combine like terms.
:::

---

### 2.4.4 – Why It Works (Another Look)

Distribution turns “**groups of a sum**” into a “**sum of groups**.”

**Word picture:** A club sells a snack bundle: each bundle has **$x$ cookies and 3 candies**. If you buy **4 bundles**, you get **$4x$ cookies and $12$ candies**:
$4(x+3)=4x+12.$

:::{.real-world title="Group purchases"}
Buying 7 “$x$-dollar passes and a $2 fee” costs $7(x+2)=7x+14$. The per-person cost ($x$) and the fixed fee (2) both get multiplied by 7.
:::

---

### 2.4.5 – Reverse It: Factoring Out a Common Factor

Distribution goes both ways. If $ab+ac = a(b+c)$, then we can **factor out** $a$.

**Examples**

1. $8x+12 = 4(2x+3)$
2. $15x-9 = 3(5x-3)$
3. $3x+6y = 3(x+2y)$

This is called **factoring** (using a **greatest common factor**, if possible).

:::{.you-try-m title="Factor the expression (reverse distribute)."}
a) $12x+18$    b) $9a-6$    c) $14y+21x$    d) $15x-9x^2$
:::

:::{.answer title="Answer"}
a) $6(2x+3)$    b) $3(3a-2)$    c) $7(2y+3x)$    d) $3x(5-3x)$
:::

---

### 2.4.6 – Check Your Work

Use a quick **substitution** to confirm equivalence.

Example: Is $5(2x-3)-(x-4)$ the same as $9x-11$?

Expand:
$5(2x-3)-(x-4)=10x-15-x+4=9x-11.$

Check $x=2$:
$5(4-3)-(2-4)=5(1)-(-2)=5+2=7 \quad \text{and} \quad 9(2)-11=18-11=7.$
They match.

:::{.gotcha title="Important: Exponents don’t distribute over addition"}
$(x+2)^2 \neq x^2+2^2$.
Correct: $(x+2)^2=(x+2)(x+2)=x^2+4x+4$.
:::

---

## 🏋️ Practice On Your Own

**Expand using the distributive property**

1. $6(x+5)$
2. $7(y-2)$
3. $4(3a+b)$
4. $10(m+0.3)$
5. $-3(p+9)$
6. $-(k-8)$

**Expand, then combine like terms**

7. $2(x+3)+5(x-1)$
8. $4y-2(3y-7)$
9. $3(a+2b)-5(2a-b)$
10. $-2(t-5)+3(t+1)$

**With decimals and fractions**

11. $0.5(8x-6)$
12. $1.2(y+5)-0.2y$
13. $\dfrac{3}{4}(4x-8)$
14. $-\dfrac{1}{2}(6a+10)$

**Factor (reverse distribute)**

15. $18x+27$
16. $20m-12$
17. $8p+12q$
18. $14x-21x^2$

**Are they equivalent? Expand/simplify and compare.**

19. $3(x+4)+2x$ and $5x+12$
20. $6-2(x+3)$ and $-2x$
21. $5(a-1)+a$ and $6a-5$
22. $4(y+2)-3(y-1)$ and $y+11$

**Challenge Problems**

23. Show two different ways to simplify $3(x+5)-2(x-1)$ (e.g., distribute-first vs. combine-inside-first if possible). Explain why both give the same result.

24. Create **two equivalent expressions** that look different: one using parentheses and one fully expanded. Explain how you know they’re equivalent.

---

:::{.answers}

**Expand using the distributive property**

1. $6x+30$
2. $7y-14$
3. $12a+4b$
4. $10m+3$
5. $-3p-27$
6. $-k+8$

**Expand, then combine like terms**

7. $2x+6+5x-5=7x+1$
8. $4y-6y+14=-2y+14$
9. $3a+6b-10a+5b=-7a+11b$
10. $-2t+10+3t+3 = t+13$

**With decimals and fractions**

11. $4x-3$
12. $1.2y+6-0.2y = 1.0y+6$ or $y+6$
13. $3x-6$
14. $-3a-5$

**Factor (reverse distribute)**

15. $9(2x+3)$
16. $4(5m-3)$
17. $4(2p+3q)$
18. $7x(2-3x)$

**Are they equivalent?**

19. yes (both $5x+12$)
20. yes (both $-2x$)
21. yes (both $6a-5$)
22. yes (both $y+11$)

:::
